Define WORD ref inv, prove translation thms
The WORD refinement invariant maps word8 to Word8 in CakeML,
and word64 to Word64. All smaller words are mapped into
appropriate versions of either word8 or word64. Words larger
than 64 bits are not supported at present.

The theory has translation theorems for n2w, w2n, and, or,
xor, and all of the shift operations. (Comparison operations
are currently missing.)

The current translation won't be able to support translation
of the 'a word type. However, it will be able to support all
instances of 'a word that fit in a word64. (I could have used
a different scheme that would allow translation of 'a word, but
any such scheme would not have mapped word8 to Word8 in CakeML
etc.) In practice this means that various compiler definitions
need to be (automatically) type instantiated before they are
handed to the translator.

translator/ml_translatorScript.sml
@@ -74,8 +74,12 @@ val NUM_def = Define `
 val BOOL_def = Define `
   BOOL b = \v:v. (v = Boolv b)`;
 
-val WORD8_def = Define `
-  WORD8 w = \v:v. (v = Litv (Word8 w))`;
+val WORD_def = Define `
+  WORD (w:'a word) =
+    \v:v. dimindex (:'a) <= 64 /\
+          (v = Litv (if dimindex (:'a) <= 8
+                     then Word8 (w2w w << (8 - dimindex (:'a)))
+                     else Word64 (w2w w << (64 - dimindex (:'a)))))`;
 
 val CHAR_def = Define`
   CHAR (c:char) = \v:v. (v = Litv (Char c))`;
@@ -228,10 +232,6 @@ val Eval_Val_BOOL_F = store_thm("Eval_Val_BOOL_F",
   \\ fs [do_app_def] \\ SIMP_TAC (srw_ss()) [Once evaluate_cases]
   \\ EVAL_TAC);
 
-val Eval_Val_WORD8 = store_thm("Eval_Val_WORD8",
-  ``!w. Eval env (Lit (Word8 w)) (WORD8 w)``,
-  SIMP_TAC (srw_ss()) [Once evaluate_cases,WORD8_def,Eval_def]);
-
 val Eval_Val_CHAR = store_thm("Eval_Val_CHAR",
   ``!c. Eval env (Lit (Char c)) (CHAR c)``,
   SIMP_TAC (srw_ss()) [CHAR_def,Eval_def,Once evaluate_cases])
@@ -272,15 +272,26 @@ val EqualityType_def = Define `
     (!x1 v1 x2 v2. abs x1 v1 /\ abs x2 v2 ==> ((v1 = v2) = (x1 = x2))) /\
     (!x1 v1 x2 v2. abs x1 v1 /\ abs x2 v2 ==> types_match v1 v2)`;
 
+val Eq_lemma = prove(
+  ``n < dimword (:'a) /\ dimindex (:α) <= k ==>
+    (n * 2n ** (k − dimindex (:α))) < 2 ** k``,
+  fs [dimword_def] \\ rw []
+  \\ fs [LESS_EQ_EXISTS] \\ rw [] \\ fs [EXP_ADD]
+  \\ simp_tac std_ss [Once MULT_COMM] \\ fs []);
+
 val EqualityType_NUM_BOOL = store_thm("EqualityType_NUM_BOOL",
   ``EqualityType NUM /\ EqualityType INT /\
-    EqualityType BOOL /\ EqualityType WORD8 /\
+    EqualityType BOOL /\ EqualityType WORD /\
     EqualityType CHAR /\ EqualityType STRING_TYPE /\
     EqualityType UNIT_TYPE``,
   EVAL_TAC \\ fs [no_closures_def,
     types_match_def, lit_same_type_def,
     stringTheory.ORD_11,mlstringTheory.explode_11]
-  \\ SRW_TAC [] [] \\ EVAL_TAC);
+  \\ SRW_TAC [] [] \\ EVAL_TAC
+  \\ fs [w2w_def] \\ Cases_on `x1` \\ Cases_on `x2`
+  \\ fs [WORD_MUL_LSL,word_mul_n2w]
+  \\ imp_res_tac Eq_lemma \\ fs []
+  \\ fs [MULT_EXP_MONO |> Q.SPECL [`p`,`1`] |> SIMP_RULE bool_ss [EVAL ``SUC 1``]]);
 
 val types_match_list_length = prove(
   ``!vs1 vs2. types_match_list vs1 vs2 ==> LENGTH vs1 = LENGTH vs2``,
@@ -784,53 +795,325 @@ val Eval_NUM_EQ_0 = store_thm("Eval_NUM_EQ_0",
   \\ `(n = 0) = (&n <= 0)` by intLib.COOPER_TAC
   \\ FULL_SIMP_TAC std_ss [Eval_INT_LESS_EQ]);
 
-(* word8 conversions *)
 
-val Eval_w82n = store_thm("Eval_w82n",
-  ``Eval env x1 (WORD8 w) ==> Eval env (App W8toInt [x1]) (NUM (w2n w))``,
-  rw[Eval_def,WORD8_def]
+(* word operations *)
+
+val Eval_word_and = store_thm("Eval_word_and",
+  ``Eval env x1 (WORD (w1:'a word)) /\
+    Eval env x2 (WORD (w2:'a word)) ==>
+    Eval env (App (Opw (if dimindex (:'a) <= 8 then W8 else W64) Andw) [x1;x2])
+      (WORD (word_and w1 w2))``,
+  rw[Eval_def,WORD_def]
   \\ rw[Once evaluate_cases,PULL_EXISTS]
   \\ rw[Once evaluate_cases,PULL_EXISTS]
   \\ rw[Once (CONJUNCT2 evaluate_cases),PULL_EXISTS]
+  \\ rw[Once (CONJUNCT2 evaluate_cases),PULL_EXISTS]
+  \\ once_rewrite_tac [METIS_PROVE [] ``b1/\b2/\b3/\b4<=>b2/\b3/\b1/\b4``]
+  \\ asm_exists_tac \\ fs [] \\ asm_exists_tac \\ fs []
+  \\ fs [empty_state_def,state_component_equality]
+  \\ fs [do_app_def,opw8_lookup_def,opw64_lookup_def]
+  \\ fs [GSYM WORD_w2w_OVER_BITWISE]);
+
+val Eval_word_or = store_thm("Eval_word_or",
+  ``Eval env x1 (WORD (w1:'a word)) /\
+    Eval env x2 (WORD (w2:'a word)) ==>
+    Eval env (App (Opw (if dimindex (:'a) <= 8 then W8 else W64) Orw) [x1;x2])
+      (WORD (word_or w1 w2))``,
+  rw[Eval_def,WORD_def]
+  \\ rw[Once evaluate_cases,PULL_EXISTS]
+  \\ rw[Once evaluate_cases,PULL_EXISTS]
+  \\ rw[Once (CONJUNCT2 evaluate_cases),PULL_EXISTS]
+  \\ rw[Once (CONJUNCT2 evaluate_cases),PULL_EXISTS]
+  \\ once_rewrite_tac [METIS_PROVE [] ``b1/\b2/\b3/\b4<=>b2/\b3/\b1/\b4``]
+  \\ asm_exists_tac \\ fs [] \\ asm_exists_tac \\ fs []
+  \\ fs [empty_state_def,state_component_equality]
+  \\ fs [do_app_def,opw8_lookup_def,opw64_lookup_def]
+  \\ fs [GSYM WORD_w2w_OVER_BITWISE]);
+
+val Eval_word_xor = store_thm("Eval_word_xor",
+  ``Eval env x1 (WORD (w1:'a word)) /\
+    Eval env x2 (WORD (w2:'a word)) ==>
+    Eval env (App (Opw (if dimindex (:'a) <= 8 then W8 else W64) Xor) [x1;x2])
+      (WORD (word_xor w1 w2))``,
+  rw[Eval_def,WORD_def]
+  \\ rw[Once evaluate_cases,PULL_EXISTS]
+  \\ rw[Once evaluate_cases,PULL_EXISTS]
+  \\ rw[Once (CONJUNCT2 evaluate_cases),PULL_EXISTS]
+  \\ rw[Once (CONJUNCT2 evaluate_cases),PULL_EXISTS]
+  \\ once_rewrite_tac [METIS_PROVE [] ``b1/\b2/\b3/\b4<=>b2/\b3/\b1/\b4``]
+  \\ asm_exists_tac \\ fs [] \\ asm_exists_tac \\ fs []
+  \\ fs [empty_state_def,state_component_equality]
+  \\ fs [do_app_def,opw8_lookup_def,opw64_lookup_def]
+  \\ fs [GSYM WORD_w2w_OVER_BITWISE]);
+
+val DISTRIB_ANY = prove(
+  ``(p * m + p * n = p * (m + n)) /\
+    (p * m + n * p = p * (m + n)) /\
+    (m * p + p * n = p * (m + n)) /\
+    (m * p + n * p = p * (m + n:num)) /\
+    (p * m - p * n = p * (m - n)) /\
+    (p * m - n * p = p * (m - n)) /\
+    (m * p - p * n = p * (m - n)) /\
+    (m * p - n * p = p * (m - n:num))``,
+  fs [LEFT_ADD_DISTRIB]);
+
+val MOD_COMMON_FACTOR_ANY = prove(
+  ``!n p q. 0 < n ∧ 0 < q ==>
+            ((n * p) MOD (n * q) = n * p MOD q) /\
+            ((p * n) MOD (n * q) = n * p MOD q) /\
+            ((n * p) MOD (q * n) = n * p MOD q) /\
+            ((p * n) MOD (q * n) = n * p MOD q)``,
+  fs [GSYM MOD_COMMON_FACTOR]);
+
+val Eval_word_add_lemma = prove(
+  ``dimindex (:'a) <= k ==>
+    (2 ** (k − dimindex (:α)) * q MOD dimword (:α)) MOD 2 ** k =
+    (2 ** (k − dimindex (:α)) * q) MOD 2 ** k``,
+  rw [] \\ fs [LESS_EQ_EXISTS]
+  \\ rw [EXP_ADD,dimword_def,MOD_COMMON_FACTOR_ANY]);
+
+val Eval_word_add = store_thm("Eval_word_add",
+  ``Eval env x1 (WORD (w1:'a word)) /\
+    Eval env x2 (WORD (w2:'a word)) ==>
+    Eval env (App (Opw (if dimindex (:'a) <= 8 then W8 else W64) Add) [x1;x2])
+      (WORD (word_add w1 w2))``,
+  rw[Eval_def,WORD_def]
+  \\ rw[Once evaluate_cases,PULL_EXISTS]
+  \\ rw[Once evaluate_cases,PULL_EXISTS]
+  \\ rw[Once (CONJUNCT2 evaluate_cases),PULL_EXISTS]
+  \\ rw[Once (CONJUNCT2 evaluate_cases),PULL_EXISTS]
+  \\ once_rewrite_tac [METIS_PROVE [] ``b1/\b2/\b3/\b4<=>b2/\b3/\b1/\b4``]
+  \\ asm_exists_tac \\ fs [] \\ asm_exists_tac \\ fs []
+  \\ fs [empty_state_def,state_component_equality]
+  \\ fs [do_app_def,opw8_lookup_def,opw64_lookup_def]
+  \\ Cases_on `w1` \\ Cases_on `w2`
+  \\ fs [word_add_n2w,w2w_def,WORD_MUL_LSL,word_mul_n2w,GSYM RIGHT_ADD_DISTRIB]
+  \\ imp_res_tac Eval_word_add_lemma \\ fs []);
+
+val Eval_word_sub_lemma = prove(
+  ``dimindex (:'a) <= k /\ n' < dimword (:α) ==>
+    (n * 2 ** (k − dimindex (:α)) +
+      (2 ** k − (n' * 2 ** (k − dimindex (:α))) MOD 2 ** k) MOD 2 ** k) MOD 2 ** k =
+    ((n + dimword (:α) − n') * 2 ** (k − dimindex (:α))) MOD 2 ** k``,
+  fs [LESS_EQ_EXISTS,dimword_def] \\ rw []
+  \\ fs [RIGHT_ADD_DISTRIB,RIGHT_SUB_DISTRIB,EXP_ADD]
+  \\ full_simp_tac std_ss [DISTRIB_ANY,MOD_COMMON_FACTOR_ANY] \\ AP_TERM_TAC
+  \\ once_rewrite_tac [EQ_SYM_EQ] \\ fs [Once (GSYM MOD_PLUS)]
+  \\ `n + 2 ** dimindex (:α) − n' = n + (2 ** dimindex (:α) − n')` by decide_tac
+  \\ pop_assum (fn th => once_rewrite_tac [th])
+  \\ fs [Once (GSYM MOD_PLUS)]);
+
+val Eval_word_sub = store_thm("Eval_word_sub",
+  ``Eval env x1 (WORD (w1:'a word)) /\
+    Eval env x2 (WORD (w2:'a word)) ==>
+    Eval env (App (Opw (if dimindex (:'a) <= 8 then W8 else W64) Sub) [x1;x2])
+      (WORD (word_sub w1 w2))``,
+  rw[Eval_def,WORD_def]
+  \\ rw[Once evaluate_cases,PULL_EXISTS]
+  \\ rw[Once evaluate_cases,PULL_EXISTS]
+  \\ rw[Once (CONJUNCT2 evaluate_cases),PULL_EXISTS]
+  \\ rw[Once (CONJUNCT2 evaluate_cases),PULL_EXISTS]
+  \\ once_rewrite_tac [METIS_PROVE [] ``b1/\b2/\b3/\b4<=>b2/\b3/\b1/\b4``]
+  \\ asm_exists_tac \\ fs [] \\ asm_exists_tac \\ fs []
+  \\ fs [empty_state_def,state_component_equality]
+  \\ fs [do_app_def,opw8_lookup_def,opw64_lookup_def]
+  \\ Cases_on `w1` \\ Cases_on `w2`
+  \\ fs [word_add_n2w,w2w_def,WORD_MUL_LSL,word_mul_n2w,GSYM RIGHT_ADD_DISTRIB]
+  \\ once_rewrite_tac [WORD_ADD_COMM]
+  \\ fs [GSYM (SIMP_CONV (srw_ss()) [word_sub_def] ``w-v:'a word``)]
+  \\ fs [word_add_n2w,w2w_def,WORD_MUL_LSL,word_mul_n2w,GSYM RIGHT_ADD_DISTRIB]
+  \\ imp_res_tac Eval_word_add_lemma
+  \\ fs [word_2comp_n2w,word_add_n2w]
+  \\ imp_res_tac Eval_word_sub_lemma \\ fs []);
+
+val w2n_w2w_8 = prove(
+  ``dimindex (:α) < 8 ==>
+    w2n ((w2w:'a word ->word8) w << (8 − dimindex (:α)) >>>
+            (8 − dimindex (:α))) = w2n w``,
+  Cases_on `w` \\ fs [w2n_lsr,w2w_def,WORD_MUL_LSL,word_mul_n2w,dimword_def]
+  \\ rw []  \\ drule (DECIDE ``n<m ==> n <= m:num``)
+  \\ fs [LESS_EQ_EXISTS] \\ fs [] \\ rw []
+  \\ fs [] \\ full_simp_tac bool_ss [GSYM (EVAL ``2n ** 8``),EXP_ADD]
+  \\ fs [MOD_COMMON_FACTOR_ANY,MULT_DIV]);
+
+val w2n_w2w_64 = prove(
+  ``dimindex (:α) < 64 ==>
+    w2n ((w2w:'a word ->word64) w << (64 − dimindex (:α)) >>>
+            (64 − dimindex (:α))) = w2n w``,
+  Cases_on `w` \\ fs [w2n_lsr,w2w_def,WORD_MUL_LSL,word_mul_n2w,dimword_def]
+  \\ rw []  \\ drule (DECIDE ``n<m ==> n <= m:num``)
+  \\ fs [LESS_EQ_EXISTS] \\ fs [] \\ rw []
+  \\ fs [] \\ full_simp_tac bool_ss [GSYM (EVAL ``2n ** 64``),EXP_ADD]
+  \\ fs [MOD_COMMON_FACTOR_ANY,MULT_DIV]);
+
+val Eval_w2n = store_thm("Eval_w2n",
+  ``Eval env x1 (WORD (w:'a word)) ==>
+    Eval env
+      (if dimindex (:'a) = 8 then
+         App (WordToInt W8) [x1]
+       else if dimindex (:'a) = 64 then
+         App (WordToInt W64) [x1]
+       else if dimindex (:'a) < 8 then
+         App (WordToInt W8) [App (Shift W8 Lsr (8 - dimindex (:'a))) [x1]]
+       else
+         App (WordToInt W64) [App (Shift W64 Lsr (64 - dimindex (:'a))) [x1]])
+      (NUM (w2n w))``,
+  rw[Eval_def,WORD_def] \\ fs []
+  \\ TRY (* takes care of = 8 and = 64 cases *)
+   (rw[Once evaluate_cases,PULL_EXISTS]
+    \\ rw[Once evaluate_cases,PULL_EXISTS]
+    \\ rw[Once (CONJUNCT2 evaluate_cases),PULL_EXISTS]
+    \\ once_rewrite_tac [METIS_PROVE [] ``b1/\b2/\b3/\b4<=>b2/\b1/\b3/\b4``]
+    \\ asm_exists_tac \\ simp[]
+    \\ fs [empty_state_def,state_component_equality]
+    \\ fs [do_app_def,NUM_def,INT_def,w2w_def]
+    \\ assume_tac w2n_lt \\ rfs [dimword_def])
+  \\ rw[Once evaluate_cases,PULL_EXISTS]
+  \\ rw[Once evaluate_cases,PULL_EXISTS]
+  \\ rw[Once (CONJUNCT2 evaluate_cases),PULL_EXISTS]
+  \\ rw[Once evaluate_cases,PULL_EXISTS]
+  \\ rw[Once (CONJUNCT2 evaluate_cases),PULL_EXISTS]
+  \\ rw[Once (CONJUNCT2 evaluate_cases),PULL_EXISTS]
   \\ once_rewrite_tac [METIS_PROVE [] ``b1/\b2/\b3/\b4<=>b2/\b1/\b3/\b4``]
-  \\ asm_exists_tac \\ simp[]
-  \\ rw[do_app_cases] \\ EVAL_TAC);
+  \\ asm_exists_tac \\ fs []
+  \\ fs [empty_state_def,state_component_equality,do_app_def]
+  \\ EVAL_TAC \\ fs [w2n_w2w_64,w2n_w2w_8]);
 
-val Eval_w82i = Q.store_thm("Eval_w82i",
-  `Eval env x1 (WORD8 w) ==>
-   Eval env (Let (SOME "i") (App W8toInt [x1])
-               (If (App (Opb Lt) [Var (Short "i"); Lit (IntLit 128)])
-                  (Var (Short "i"))
-                  (App (Opn Minus) [Var (Short "i"); Lit (IntLit 256)])))
-     (INT (w2i w))`,
-  `w2i w = let i = & (w2n w) in if i < 128 then i else i - 256`
-       by fs [integer_wordTheory.w2i_eq_w2n]
-  \\ full_simp_tac std_ss [] \\ strip_tac
-  \\ match_mp_tac (GEN_ALL Eval_Let)
-  \\ imp_res_tac Eval_w82n \\ fs [NUM_def]
-  \\ asm_exists_tac \\ fs [] \\ rpt strip_tac
-  \\ match_mp_tac (GEN_ALL (MP_CANON Eval_If))
-  \\ rpt (qexists_tac `T`) \\ rpt strip_tac
-  \\ TRY (match_mp_tac (MP_CANON Eval_INT_SUB))
-  \\ TRY (match_mp_tac (MP_CANON Eval_NUM_LESS))
-  \\ fs [NUM_def,Eval_Var_SIMP,Eval_Val_INT]);
-
-val Eval_i2w8 = Q.store_thm("Eval_i2w8",
-  `Eval env x1 (INT i) ==> Eval env (App W8fromInt [x1]) (WORD8 (i2w i))`,
-  rw[Eval_def,INT_def]
+val Eval_n2w = store_thm("Eval_n2w",
+  ``dimindex (:'a) <= 64 ==>
+    Eval env x1 (NUM n) ==>
+    Eval env
+      (if dimindex (:'a) = 8 then
+         App (WordFromInt W8) [x1]
+       else if dimindex (:'a) = 64 then
+         App (WordFromInt W64) [x1]
+       else if dimindex (:'a) < 8 then
+         App (Shift W8 Lsl (8 - dimindex (:'a))) [App (WordFromInt W8) [x1]]
+       else
+         App (Shift W64 Lsl (64 - dimindex (:'a))) [App (WordFromInt W64) [x1]])
+      (WORD ((n2w n):'a word))``,
+  rw[Eval_def,WORD_def] \\ fs [] \\ rfs []
+  \\ TRY (* takes care of = 8 and = 64 cases *)
+   (rw[Once evaluate_cases,PULL_EXISTS]
+    \\ rw[Once evaluate_cases,PULL_EXISTS]
+    \\ rw[Once (CONJUNCT2 evaluate_cases),PULL_EXISTS]
+    \\ once_rewrite_tac [METIS_PROVE [] ``b1/\b2/\b3<=>b2/\b1/\b3``]
+    \\ asm_exists_tac \\ simp[]
+    \\ fs [empty_state_def,state_component_equality]
+    \\ fs [do_app_def,NUM_def,INT_def,w2w_def,integer_wordTheory.i2w_def]
+    \\ fs [dimword_def] \\ NO_TAC)
   \\ rw[Once evaluate_cases,PULL_EXISTS]
   \\ rw[Once evaluate_cases,PULL_EXISTS]
-  \\ rw[Once (CONJUNCT2 evaluate_cases)]
-  \\ rw[do_app_cases,PULL_EXISTS,WORD8_def]
-  \\ ONCE_REWRITE_TAC[CONJ_COMM]
-  \\ asm_exists_tac \\ rw[]
-  \\ EVAL_TAC);
+  \\ rw[Once (CONJUNCT2 evaluate_cases),PULL_EXISTS]
+  \\ rw[Once evaluate_cases,PULL_EXISTS]
+  \\ rw[Once (CONJUNCT2 evaluate_cases),PULL_EXISTS]
+  \\ rw[Once (CONJUNCT2 evaluate_cases),PULL_EXISTS]
+  \\ once_rewrite_tac [METIS_PROVE [] ``b1/\b2/\b3/\b4<=>b2/\b1/\b3/\b4``]
+  \\ asm_exists_tac \\ fs []
+  \\ fs [empty_state_def,state_component_equality,do_app_def,NUM_def,INT_def]
+  \\ fs [shift8_lookup_def,shift64_lookup_def,
+         w2w_def,integer_wordTheory.i2w_def,WORD_MUL_LSL,word_mul_n2w]
+  \\ rw [dimword_def] \\ TRY (drule (DECIDE ``n<m ==> n <= m:num``))
+  \\ fs [LESS_EQ_EXISTS] \\ fs [] \\ rw [] \\ fs []
+  \\ full_simp_tac bool_ss
+       [GSYM (EVAL ``2n ** 8``),GSYM (EVAL ``2n ** 64``),EXP_ADD]
+  \\ fs [MOD_COMMON_FACTOR_ANY,MULT_DIV]);
 
-val Eval_n2w8 = Q.store_thm("Eval_n2w8",
-  `Eval env x1 (NUM n) ==> Eval env (App W8fromInt [x1]) (WORD8 (n2w n))`,
-  rw[NUM_def]
-  \\ drule Eval_i2w8
-  \\ simp[integer_wordTheory.i2w_def]);
+val Eval_word_lsl = store_thm("Eval_word_lsl",
+  ``Eval env x1 (WORD (w1:'a word)) ==>
+    Eval env (App (Shift (if dimindex (:'a) <= 8 then W8 else W64) Lsl n) [x1])
+      (WORD (word_lsl w1 n))``,
+  rw[Eval_def,WORD_def]
+  \\ rw[Once evaluate_cases,PULL_EXISTS]
+  \\ rw[Once evaluate_cases,PULL_EXISTS]
+  \\ rw[Once (CONJUNCT2 evaluate_cases),PULL_EXISTS]
+  \\ rw[Once (CONJUNCT2 evaluate_cases),PULL_EXISTS]
+  \\ once_rewrite_tac [METIS_PROVE [] ``b1/\b2/\b3<=>b2/\b3/\b1``]
+  \\ asm_exists_tac \\ fs []
+  \\ fs [empty_state_def,state_component_equality]
+  \\ fs [LESS_EQ_EXISTS]
+  \\ fs [do_app_def,shift8_lookup_def,shift64_lookup_def]
+  \\ fs [fcpTheory.CART_EQ,word_lsl_def,fcpTheory.FCP_BETA,w2w] \\ rw []
+  \\ Cases_on `w1 ' (i − (n + p))` \\ fs []);
+
+val Eval_word_lsr = store_thm("Eval_word_lsr",
+  ``Eval env x1 (WORD (w1:'a word)) ==>
+    Eval env (let w = (if dimindex (:'a) <= 8 then W8 else W64) in
+              let k = (if dimindex (:'a) <= 8 then 8 else 64) - dimindex(:'a) in
+                if dimindex (:'a) = 8 \/ dimindex (:'a) = 64 then
+                  App (Shift w Lsr n) [x1]
+                else
+                  App (Shift w Lsl k) [App (Shift w Lsr (n+k)) [x1]])
+      (WORD (word_lsr w1 n))``,
+  rw[Eval_def,WORD_def]
+  \\ TRY (* takes care of = 8 and = 64 cases *)
+   (rw[Once evaluate_cases,PULL_EXISTS]
+    \\ rw[Once evaluate_cases,PULL_EXISTS]
+    \\ rw[Once (CONJUNCT2 evaluate_cases),PULL_EXISTS]
+    \\ rw[Once (CONJUNCT2 evaluate_cases),PULL_EXISTS]
+    \\ once_rewrite_tac [METIS_PROVE [] ``b1/\b2/\b3<=>b2/\b3/\b1``]
+    \\ asm_exists_tac \\ fs []
+    \\ fs [empty_state_def,state_component_equality]
+    \\ fs [do_app_def,shift8_lookup_def,shift64_lookup_def]
+    \\ fs [fcpTheory.CART_EQ,word_lsr_def,fcpTheory.FCP_BETA,w2w] \\ rw []
+    \\ eq_tac \\ rfs [w2w] \\ rw [] \\ rfs [w2w] \\ NO_TAC)
+  \\ fs []
+  \\ rw[Once evaluate_cases,PULL_EXISTS]
+  \\ rw[Once evaluate_cases,PULL_EXISTS]
+  \\ rw[Once (CONJUNCT2 evaluate_cases),PULL_EXISTS]
+  \\ rw[Once evaluate_cases,PULL_EXISTS]
+  \\ rw[Once (CONJUNCT2 evaluate_cases),PULL_EXISTS]
+  \\ rw[Once (CONJUNCT2 evaluate_cases),PULL_EXISTS]
+  \\ once_rewrite_tac [METIS_PROVE [] ``b1/\b2/\b3/\b4<=>b2/\b1/\b3/\b4``]
+  \\ asm_exists_tac \\ fs []
+  \\ fs [empty_state_def,state_component_equality]
+  \\ fs [LESS_EQ_EXISTS,do_app_def]
+  \\ fs [shift8_lookup_def,shift64_lookup_def]
+  \\ fs [fcpTheory.CART_EQ,word_lsr_def,word_lsl_def,fcpTheory.FCP_BETA,w2w]
+  \\ rw [] \\ fs [] \\ eq_tac \\ rw [] \\ fs []
+  \\ fs [fcpTheory.FCP_BETA,w2w]
+  \\ imp_res_tac (DECIDE  ``p <= i ==> (i - p + n = (i + n) - p:num)``) \\ fs []
+  \\ TRY (`i − p + (n + p) < 8` by decide_tac \\ fs [fcpTheory.FCP_BETA,w2w])
+  \\ TRY (`i − p + (n + p) < 64` by decide_tac \\ fs [fcpTheory.FCP_BETA,w2w]));
+
+val Eval_word_asr = store_thm("Eval_word_lsr",
+  ``Eval env x1 (WORD (w1:'a word)) ==>
+    Eval env (let w = (if dimindex (:'a) <= 8 then W8 else W64) in
+              let k = (if dimindex (:'a) <= 8 then 8 else 64) - dimindex(:'a) in
+                if dimindex (:'a) = 8 \/ dimindex (:'a) = 64 then
+                  App (Shift w Asr n) [x1]
+                else
+                  App (Shift w Lsl k) [App (Shift w Asr (n+k)) [x1]])
+      (WORD (word_asr w1 n))``,
+  rw[Eval_def,WORD_def]
+  \\ TRY (* takes care of = 8 and = 64 cases *)
+   (rw[Once evaluate_cases,PULL_EXISTS]
+    \\ rw[Once evaluate_cases,PULL_EXISTS]
+    \\ rw[Once (CONJUNCT2 evaluate_cases),PULL_EXISTS]
+    \\ rw[Once (CONJUNCT2 evaluate_cases),PULL_EXISTS]
+    \\ once_rewrite_tac [METIS_PROVE [] ``b1/\b2/\b3<=>b2/\b3/\b1``]
+    \\ asm_exists_tac \\ fs []
+    \\ fs [empty_state_def,state_component_equality]
+    \\ fs [do_app_def,shift8_lookup_def,shift64_lookup_def]
+    \\ fs [fcpTheory.CART_EQ,word_asr_def,fcpTheory.FCP_BETA,w2w] \\ rw []
+    \\ fs [word_msb_def] \\ rfs [w2w] \\ rw [] \\ rfs [w2w] \\ NO_TAC)
+  \\ fs []
+  \\ rw[Once evaluate_cases,PULL_EXISTS]
+  \\ rw[Once evaluate_cases,PULL_EXISTS]
+  \\ rw[Once (CONJUNCT2 evaluate_cases),PULL_EXISTS]
+  \\ rw[Once evaluate_cases,PULL_EXISTS]
+  \\ rw[Once (CONJUNCT2 evaluate_cases),PULL_EXISTS]
+  \\ rw[Once (CONJUNCT2 evaluate_cases),PULL_EXISTS]
+  \\ once_rewrite_tac [METIS_PROVE [] ``b1/\b2/\b3/\b4<=>b2/\b1/\b3/\b4``]
+  \\ asm_exists_tac \\ fs []
+  \\ fs [empty_state_def,state_component_equality]
+  \\ fs [LESS_EQ_EXISTS,do_app_def]
+  \\ fs [shift8_lookup_def,shift64_lookup_def]
+  \\ fs [fcpTheory.CART_EQ,word_asr_def,word_lsl_def,fcpTheory.FCP_BETA,w2w]
+  \\ rw [] \\ fs [] \\ eq_tac \\ rw [] \\ fs []
+  \\ fs [fcpTheory.FCP_BETA,w2w,word_msb_def]
+  \\ imp_res_tac (DECIDE ``8 = k ==> 7 = k - 1n``) \\ fs []
+  \\ imp_res_tac (DECIDE ``64 = k ==> 63 = k - 1n``) \\ fs []);
 
 (* list definition *)
 
